\documentclass {article}

\usepackage {amsthm}
\usepackage {amssymb}
\usepackage {amsmath}

\title {The Quadratic Formula}
\date  {}

\begin {document}
    \maketitle 
    Start with the general quadratic equation:
    \[ ax^2 + bx + c = 0 \]
    We can complete the square to derive the quadratic formula:
    \begin {align*}
        x^2 + \frac{b}{a} \cdot x + \frac{c}{a} &= 0 \\
        x^2 + \frac{b}{a} \cdot x &= -\frac{c}{a} \\
        x^2 + \frac{b}{a} \cdot x + \left( \frac{b}{2a} \right)^2 &= \left( \frac{b}{2a} \right)^2 - \frac{c}{a} \\
        \left( x + \frac{b}{2a} \right)^2 &= \frac{b^2}{4a^2} - \frac{c}{a} \\
        \left( x + \frac{b}{2a} \right)^2 &= \frac{b^2}{4a^2} - \frac{4ac}{4a^2} \\
        x + \frac{b}{2a} &= \pm \sqrt{\frac{b^2 - 4ac}{4a^2}} \\
        x + \frac{b}{2a} &= \pm \frac{\sqrt{b^2 - 4ac}}{2a} \\
        x &= \frac{-b \pm \sqrt{b^2 - 4ac}}{2a}
    \end {align*}
\end {document}
